(Mostly) replaced JSON’s Unicode module

src/Unicode/UnicodeStrings.dfy
@@ -4,15 +4,36 @@
 
 include "../BoundedInts.dfy"
 include "../Wrappers.dfy"
+include "../Collections/Sequences/Seq.dfy"
 include "Utf8EncodingForm.dfy"
+include "Utf8EncodingScheme.dfy"
 include "Utf16EncodingForm.dfy"
 
-abstract module AbstractUnicodeStrings {
+abstract module {:options "-functionSyntax:4"} AbstractUnicodeStrings {
+
+  import Seq
 
   import opened Wrappers
   import opened BoundedInts
+  import opened Utf8EncodingScheme
 
-  function ToUTF8(s: string): Option<seq<uint8>>
+  function ToUTF8Checked(s: string): Option<seq<uint8>>
 
-  function FromUTF8(bs: seq<uint8>): Option<string>
+  function ASCIIToUTF8(s: string): seq<uint8> 
+    requires forall i | 0 <= i < |s| :: 0 <= s[i] as int < 128
+  {
+    Seq.Map(c requires 0 <= c as int < 128 => c as uint8, s)
+  }
+
+  function FromUTF8Checked(bs: seq<uint8>): Option<string>
+
+  function ToUTF16Checked(s: string): Option<seq<uint16>>
+
+  function BMPToUTF16(s: string): seq<uint16> 
+    requires forall i | 0 <= i < |s| :: 0 <= s[i] as int < 0x1_0000
+  {
+    Seq.Map(c requires 0 <= c as int < 0x1_0000 => c as uint16, s)
+  }
+
+  function FromUTF16Checked(bs: seq<uint16>): Option<string>
 }
