src/Unicode/UnicodeStringsWithoutUnicodeChar.dfy
@@ -4,26 +4,46 @@ include "UnicodeStrings.dfy"
 include "../Wrappers.dfy"
 include "../Collections/Sequences/Seq.dfy"
 
-module UnicodeStrings refines AbstractUnicodeStrings {
+module {:options "-functionSyntax:4"} UnicodeStrings refines AbstractUnicodeStrings {
 
   import Unicode
   import Utf8EncodingForm
   import Utf16EncodingForm 
-  import Seq
   
-  function ToUTF8(s: string): Option<seq<uint8>> {
+  predicate IsWellFormedString(s: string)
+    ensures |s| == 0 ==> IsWellFormedString(s) 
+  {
+    Utf16EncodingForm.IsWellFormedCodeUnitSequence(Seq.Map(c => c as Utf16EncodingForm.CodeUnit, s)) 
+  }
+
+  function ToUTF8Checked(s: string): Option<seq<uint8>> {
     var asCodeUnits := Seq.Map(c => c as Utf16EncodingForm.CodeUnit, s);
     var utf32 :- Utf16EncodingForm.DecodeCodeUnitSequenceChecked(asCodeUnits);
     var asUtf8CodeUnits := Utf8EncodingForm.EncodeScalarSequence(utf32);
-    var asBytes := Seq.Map(cu => cu as uint8, asUtf8CodeUnits);
-    Some(asBytes)
+    Some(Utf8EncodingScheme.Serialize(asUtf8CodeUnits))
   }
 
-  function FromUTF8(bs: seq<uint8>): Option<string> {
+  function {:vcs_split_on_every_assert} FromUTF8Checked(bs: seq<uint8>): Option<string> {
     var asCodeUnits := Seq.Map(c => c as Utf8EncodingForm.CodeUnit, bs);
     var utf32 :- Utf8EncodingForm.DecodeCodeUnitSequenceChecked(asCodeUnits);
     var asUtf16CodeUnits := Utf16EncodingForm.EncodeScalarSequence(utf32);
     var asChars := Seq.Map(cu => cu as char, asUtf16CodeUnits);
+    assert Seq.Map(c => c as Utf16EncodingForm.CodeUnit, asChars) == asUtf16CodeUnits;
+    assert Utf16EncodingForm.IsWellFormedCodeUnitSequence(Seq.Map(c => c as Utf16EncodingForm.CodeUnit, asChars));
     Some(asChars)
+  }
+
+  function ToUTF16Checked(s: string): Option<seq<uint16>> {
+    if Utf16EncodingForm.IsWellFormedCodeUnitSequence(Seq.Map(c => c as Utf16EncodingForm.CodeUnit, s)) then
+      Some(Seq.Map(c => c as uint16, s))
+    else
+      None
+  }
+
+  function FromUTF16Checked(bs: seq<uint16>): Option<string> {
+    if Utf16EncodingForm.IsWellFormedCodeUnitSequence(Seq.Map(c => c as Utf16EncodingForm.CodeUnit, bs)) then
+      Some(Seq.Map(c => c as char, bs))
+    else
+      None
   }
 }
